pulse/src/ocaml/plugin/generated/Pulse_Syntax_Pure.ml
@@ -575,6 +575,19 @@ let (tm_inv :
            (Pulse_RuntimeUtils.range_of_term p))
 let (tm_all_inames : Pulse_Syntax_Base.term) =
   tm_fvar (Pulse_Syntax_Base.as_fv Pulse_Reflection_Util.all_inames_lid)
+let (tm_add_inv :
+  FStar_Reflection_Types.term ->
+    FStar_Reflection_Types.term -> FStar_Reflection_Types.term)
+  =
+  fun is ->
+    fun iref ->
+      let h =
+        FStar_Reflection_V2_Builtins.pack_ln
+          (FStar_Reflection_V2_Data.Tv_FVar
+             (FStar_Reflection_V2_Builtins.pack_fv
+                Pulse_Reflection_Util.add_inv_lid)) in
+      FStar_Reflection_V2_Derived.mk_app h
+        [Pulse_Reflection_Util.ex is; Pulse_Reflection_Util.ex iref]
 type ('tv, 't) is_view_of = Obj.t
 let rec (inspect_term : FStar_Reflection_Types.term -> term_view) =
   fun t ->
